eve/Src/framework/eiffel2boogie/translation/custom/e2b_custom_integer_call_handler.e
@@ -17,6 +17,7 @@ feature -- Status report
 	is_handling_call (a_target_type: TYPE_A; a_feature: FEATURE_I): BOOLEAN
 			-- <Precursor>
 		do
+			Result := a_target_type.is_numeric
 		end
 
 feature -- Basic operations
@@ -24,11 +25,52 @@ feature -- Basic operations
 	handle_routine_call_in_body (a_translator: E2B_BODY_EXPRESSION_TRANSLATOR; a_feature: FEATURE_I; a_parameters: BYTE_LIST [PARAMETER_B])
 			-- <Precursor>
 		do
+			handle_routine_call (a_translator, a_feature, a_parameters)
 		end
 
 	handle_routine_call_in_contract (a_translator: E2B_CONTRACT_EXPRESSION_TRANSLATOR; a_feature: FEATURE_I; a_parameters: BYTE_LIST [PARAMETER_B])
 			-- <Precursor>
 		do
+			handle_routine_call (a_translator, a_feature, a_parameters)
+		end
+
+feature -- Implementation
+
+	handle_routine_call (a_translator: E2B_EXPRESSION_TRANSLATOR; a_feature: FEATURE_I; a_parameters: BYTE_LIST [PARAMETER_B])
+			-- <Precursor>
+		local
+			l_name: STRING
+			l_fname: STRING
+		do
+			l_name := a_feature.feature_name
+			if l_name.same_string ("truncated_to_integer") then
+				l_fname := "real_to_integer_32"
+			elseif l_name.same_string ("truncated_to_integer_64") then
+				l_fname := "real_to_integer_64"
+			elseif l_name.same_string ("to_natural_8") or l_name.same_string ("as_natural_8") then
+				l_fname := "int_to_natural_8"
+			elseif l_name.same_string ("to_natural_16") or l_name.same_string ("as_natural_16") then
+				l_fname := "int_to_natural_16"
+			elseif l_name.same_string ("to_natural_32") or l_name.same_string ("as_natural_32") then
+				l_fname := "int_to_natural_32"
+			elseif l_name.same_string ("to_natural_64") or l_name.same_string ("as_natural_64") then
+				l_fname := "int_to_natural_64"
+			elseif l_name.same_string ("to_integer_8") or l_name.same_string ("as_integer_8") then
+				l_fname := "int_to_integer_8"
+			elseif l_name.same_string ("to_integer_16") or l_name.same_string ("as_integer_16") then
+				l_fname := "int_to_integer_16"
+			elseif l_name.same_string ("to_integer_32") or l_name.same_string ("as_integer_32") then
+				l_fname := "int_to_integer_32"
+			elseif l_name.same_string ("to_integer_64") or l_name.same_string ("as_integer_64") then
+				l_fname := "int_to_integer_64"
+			else
+				l_fname := Void
+			end
+			if l_fname /= Void then
+				a_translator.set_last_expression (factory.function_call (l_fname, << a_translator.current_target >>, types.generic_type))
+			else
+				a_translator.process_routine_call (a_feature, a_parameters)
+			end
 		end
 
 end
