eve/Src/framework/eiffel2boogie/translation/custom/e2b_custom_ownership_handler.e
@@ -10,6 +10,8 @@ inherit
 
 	E2B_CUSTOM_CALL_HANDLER
 
+	E2B_CUSTOM_NESTED_HANDLER
+
 	SHARED_WORKBENCH
 
 feature -- Status report
@@ -17,9 +19,24 @@ feature -- Status report
 	is_handling_call (a_target_type: TYPE_A; a_feature: FEATURE_I): BOOLEAN
 			-- <Precursor>
 		do
-			Result :=
-				a_feature.written_in = system.any_id and then
-				feature_names.has (a_feature.feature_name)
+			Result := a_feature.written_in = system.any_id and
+				(builtin_any_features.has (a_feature.feature_name) or
+				set_access.has (a_feature.feature_name) or
+				set_setter.has (a_feature.feature_name))
+		end
+
+	is_handling_nested (a_nested: NESTED_B): BOOLEAN
+			-- Is this handler handling the call?
+		do
+			if
+				not a_nested.target.type.is_like and then
+				a_nested.target.type.base_class /= Void and then
+				a_nested.target.type.base_class.class_id = system.tuple_id
+			then
+				if attached {FEATURE_B} a_nested.message as f then
+					Result := f.feature_name.same_string ("to_ownership_set")
+				end
+			end
 		end
 
 feature -- Basic operations
@@ -28,9 +45,27 @@ feature -- Basic operations
 			-- <Precursor>
 		local
 			l_name: STRING
+			l_assign: IV_ASSIGNMENT
+			l_call: IV_PROCEDURE_CALL
 		do
 			l_name := a_feature.feature_name
-			a_translator.process_builtin_routine_call (a_feature, a_parameters, l_name)
+			if builtin_any_features.has (l_name) then
+				a_translator.process_builtin_routine_call (a_feature, a_parameters, l_name)
+			elseif set_access.has (l_name) then
+				a_translator.set_last_expression (factory.heap_current_access (a_translator.entity_mapping, l_name))
+			else
+				check set_setter.has (l_name) end
+				l_name := l_name.substring (5, l_name.count)
+				a_translator.process_builtin_routine_call (a_feature, a_parameters, "xyz")
+				l_call ?= a_translator.side_effect.last
+				a_translator.side_effect.finish
+				a_translator.side_effect.remove
+				create l_assign.make (
+					factory.heap_current_access (a_translator.entity_mapping, l_name),
+					l_call.arguments.i_th (2))
+				a_translator.set_last_expression (Void)
+				a_translator.side_effect.extend (l_assign)
+			end
 		end
 
 	handle_routine_call_in_contract (a_translator: E2B_CONTRACT_EXPRESSION_TRANSLATOR; a_feature: FEATURE_I; a_parameters: BYTE_LIST [PARAMETER_B])
@@ -39,11 +74,67 @@ feature -- Basic operations
 			l_name: STRING
 		do
 			l_name := a_feature.feature_name
-			a_translator.process_builtin_routine_call (a_feature, a_parameters, l_name)
+			if builtin_any_features.has (l_name) then
+				a_translator.process_builtin_routine_call (a_feature, a_parameters, l_name)
+			elseif set_access.has (l_name) then
+				a_translator.set_last_expression (factory.heap_current_access (a_translator.entity_mapping, l_name))
+			else
+					-- cannot happen
+				check False end
+			end
 		end
 
-	feature_names: ARRAY [STRING]
-			-- List of feature names.
+	handle_nested_in_body (a_translator: E2B_BODY_EXPRESSION_TRANSLATOR; a_nested: NESTED_B)
+			-- <Precursor>
+		do
+			handle_nested (a_translator, a_nested)
+		end
+
+	handle_nested_in_contract (a_translator: E2B_CONTRACT_EXPRESSION_TRANSLATOR; a_nested: NESTED_B)
+			-- <Precursor>
+		do
+			handle_nested (a_translator, a_nested)
+		end
+
+	handle_nested (a_translator: E2B_EXPRESSION_TRANSLATOR; a_nested: NESTED_B)
+			-- Handle `a_nested'.
+		local
+			l_tuple: TUPLE_CONST_B
+			l_exprs: LINKED_LIST [IV_EXPRESSION]
+			l_expr: IV_EXPRESSION
+		do
+			if attached {ACCESS_EXPR_B} a_nested.target as x then
+				l_tuple ?= x.expr
+			end
+			check l_tuple /= Void end
+			create l_exprs.make
+			across l_tuple.expressions as i loop
+				i.item.process (a_translator)
+				l_exprs.extend (a_translator.last_expression)
+			end
+			if l_exprs.is_empty then
+				a_translator.set_last_expression (
+					factory.function_call ("Set#Empty", Void, types.set (types.ref)))
+			else
+				from
+					l_exprs.start
+					l_expr := factory.function_call ("Set#Singleton", << l_exprs.item >>, types.set (types.ref))
+					l_exprs.forth
+				until
+					l_exprs.after
+				loop
+					l_expr := factory.function_call (
+						"Set#UnionOne",
+						<< l_expr, l_exprs.item >>,
+						types.set (types.ref))
+					l_exprs.forth
+				end
+				a_translator.set_last_expression (l_expr)
+			end
+		end
+
+	builtin_any_features: ARRAY [STRING]
+			-- List of builtin names.
 		once
 			Result := <<
 				"wrap",
@@ -52,6 +143,30 @@ feature -- Basic operations
 				"is_wrapped",
 				"is_free",
 				"is_open"
+			>>
+			Result.compare_objects
+		end
+
+	set_access: ARRAY [STRING]
+			-- List of feature names.
+		once
+			Result := <<
+				"owner",
+				"owns",
+				"depends",
+				"dependants"
+			>>
+			Result.compare_objects
+		end
+
+	set_setter: ARRAY [STRING]
+			-- List of feature names.
+		once
+			Result := <<
+				"set_owner",
+				"set_owns",
+				"set_depends",
+				"set_dependants"
 			>>
 			Result.compare_objects
 		end
