eve/Src/framework/eiffel2boogie/translation/pool/e2b_tu_invariant_function.e
@@ -1,0 +1,45 @@
+note
+	description: "Summary description for {E2B_TU_INVARIANT_FUNCTION}."
+	author: ""
+	date: "$Date$"
+	revision: "$Revision$"
+
+class
+	E2B_TU_INVARIANT_FUNCTION
+
+inherit
+
+	E2B_TRANSLATION_UNIT
+
+create
+	make
+
+feature {NONE} -- Implementation
+
+	make (a_type: TYPE_A)
+			-- TODO
+		do
+			type := a_type
+			id := "inv/" + type_id (a_type)
+		end
+
+feature -- Access
+
+	type: TYPE_A
+			-- Context type of routine to be translated.
+
+	id: STRING
+			-- <Precursor>
+
+feature -- Basic operations
+
+	translate
+			-- <Precursor>
+		local
+			l_translator: E2B_TYPE_TRANSLATOR
+		do
+			create l_translator
+			l_translator.translate_invariant_function (type)
+		end
+
+end
