eve/Src/library/base/eve/ownership_set.e
@@ -1,0 +1,29 @@
+class OWNERSHIP_SET
+
+inherit
+
+	ANY
+		redefine
+			default_create
+		end
+
+create
+	default_create,
+	make_from_tuple,
+	make_from_array
+
+feature
+
+	default_create
+		do
+		end
+
+	make_from_tuple (a_tuple: TUPLE)
+		do
+		end
+
+	make_from_array (a_array: ARRAY [ANY])
+		do
+		end
+
+end
